compiler/backend/bvi_to_dataScript.sml
@@ -64,123 +64,144 @@ Proof
   fs[op_requires_names_eqn]
 QED
 
-val iAssign_def = Define `
-  iAssign arch_size n1 op vs live env =
-    if op_requires_names op then
-      let xs = SOME (list_to_num_set (vs++live++env)) in
-        if op = Greater then
-          Assign n1 Less (REVERSE vs) xs
-        else if op = GreaterEq then
-          Assign n1 LessEq (REVERSE vs) xs
-        else
-          Assign n1 op vs xs
-    else
-      let k = op_space_req op (LENGTH vs) arch_size in
-        if k = 0 then Assign n1 op vs NONE
-          else Seq (MakeSpace k (list_to_num_set (vs++live++env)))
-                   (Assign n1 op vs NONE)`;
-
 val _ = Parse.hide"tail";
 
-val compile_def = tDefine "compile" `
-  (compile _ (n:num) (env:num list) tail live [] =
-    (Skip,[]:num list,n)) /\
-  (compile arch_size n env tail live (x::y::xs) =
-     let (c1,v1,n1) = compile arch_size n env F live [x] in
-     let (c2,vs,n2) = compile arch_size n1 env F (HD v1::live) (y::xs) in
-       (Seq c1 c2, HD v1 :: vs, n2)) /\
-  (compile _ n env tail live [(Var v):bvi$exp] =
+Definition pure_enough_def:
+  (pure_enough (closLang$FFI _) = F) /\
+  (pure_enough Install = F) /\
+  (pure_enough (CopyByte _) = F) /\
+  (pure_enough DerefByte = F)/\
+  (pure_enough UpdateByte = F) /\
+  (pure_enough RefArray = F) /\
+  (pure_enough (RefByte _) = F) /\
+  (pure_enough SetGlobalsPtr = F) /\
+  (pure_enough GlobalsPtr = F) /\
+  (pure_enough AllocGlobal = F) /\
+  (pure_enough (SetGlobal _) = F) /\
+  (pure_enough (Global _) = F) /\
+  (pure_enough Ref = F) /\
+  (pure_enough Length = F) /\
+  (pure_enough LengthByte = F) /\
+  (pure_enough _ = T)
+End
+
+Definition compile_op_def:
+  compile_op op vs arch_size =
+    let p = pure_enough op in
+      if op_requires_names op then
+        if op = closLang$Greater then (closLang$Less, REVERSE vs, T, 0, p) else
+        if op = closLang$GreaterEq then (LessEq, REVERSE vs, T, 0, p) else
+          (op, vs, T, 0, p)
+      else (op, vs, F, op_space_req op (LENGTH vs) arch_size, p)
+End
+
+Definition compile_assign_def:
+  compile_assign acc op vs =
+    let (n,live,cache,arch_size) = acc in
+    let (new_op,new_vs,names,k,p) = compile_op op vs arch_size in
+      if p /\ IS_SOME (ALOOKUP cache (new_op,new_vs)) then
+        (Skip,THE (ALOOKUP cache (new_op,new_vs)),acc)
+      else
+         let c0 = Assign n new_op new_vs (if names then SOME live else NONE) in
+         let c1 = (if k = 0 then c0 else Seq (MakeSpace k live) c0) in
+         let new_cache = if p then ((new_op,new_vs),n) :: cache else cache in
+         let new_acc = (n+1,insert n () live,new_cache,arch_size) in
+           (c1,n,new_acc)
+End
+
+Definition compile_def:
+  (compile acc (env:num list) tail [] =
+    (Skip,[]:num list,acc)) /\
+  (compile acc env tail (x::y::xs) =
+     let (c1,v1,acc1) = compile acc env F [x] in
+     let (c2,vs,acc2) = compile acc1 env F (y::xs) in
+       (Seq c1 c2, HD v1 :: vs, acc2)) /\
+  (compile acc env tail [(Var v):bvi$exp] =
      let var = any_el v env 0n in
-     if tail
-     then (Return var, [n], n+1)
-     else (Skip, [var], MAX n (var+1))) /\
-  (compile arch_size n env tail live [If x1 x2 x3] =
-     let (c1,v1,n1) = compile arch_size n env F live [x1] in
-     let (c2,v2,n2) = compile arch_size n1 env tail live [x2] in
-     let (c3,v3,n3) = compile arch_size n2 env tail live [x3] in
+       if tail then (Return var, [var], acc)
+               else (Skip, [var], acc)) /\
+  (compile acc env tail [If x1 x2 x3] =
+     let (c1,v1,acc1) = compile acc env F [x1] in
+     let (c2,v2,acc2) = compile acc1 env tail [x2] in
+     let (c3,v3,acc3) = compile acc1 env tail [x3] in
        if tail then
-         (Seq c1 (If (HD v1) c2 c3),[n3],n3+1)
+         (Seq c1 (If (HD v1) c2 c3),v2,acc1)
        else
-         (Seq c1 (If (HD v1) (Seq c2 (Move n3 (HD v2)))
-                             (Seq c3 (Move n3 (HD v3)))),[n3],n3+1)) /\
-  (compile arch_size n env tail live [Let xs x2] =
-     let (c1,vs,n1) = compile arch_size n env F live xs in
-     let (c2,v2,n2) = compile arch_size n1 (vs ++ env) tail live [x2] in
-       (Seq c1 c2, v2, n2)) /\
-  (compile arch_size n env tail live [Raise x1] =
-     let (c1,v1,n1) = compile arch_size n env F live [x1] in
-       (Seq c1 (Raise (HD v1)), v1, n1)) /\
-  (compile arch_size n env tail live [Op op xs] =
-     let (c1,vs,n1) = compile arch_size n env F live xs in
-     let c2 = Seq c1 (iAssign arch_size n1 op (REVERSE vs) live env) in
-       (if tail then Seq c2 (Return n1) else c2, [n1], n1+1)) /\
-  (compile arch_size n env tail live [Tick x1] =
-     let (c1,v1,n1) = compile arch_size n env tail live [x1] in
-       (Seq Tick c1, v1, n1)) /\
-  (compile arch_size n env tail live [Call ticks dest xs NONE] =
-     let (c1,vs,n1) = compile arch_size n env F live xs in
-     let ret = (if tail then NONE
-                else SOME (n1, list_to_num_set (live ++ env))) in
-       (Seq c1 (mk_ticks ticks (Call ret dest vs NONE)), [n1], n1+1)) /\
-  (compile arch_size n env tail live [Call ticks dest xs (SOME handler)] =
-     let (c1,vs,n1) = compile arch_size n env F live xs in
-     let (c2,v,n2) = compile arch_size (n1+1) (n1::env) F live [handler] in
-     let ret = SOME (n2, list_to_num_set (live ++ env)) in
-     let c3 = (if tail then Return n2 else Skip) in
-       (Seq c1 (mk_ticks ticks (Seq (Call ret dest vs (SOME (n1,Seq c2 (Move n2 (HD v))))) c3)), [n2], n2+1))`
- (WF_REL_TAC `measure (exp2_size o SND o SND o SND o SND o SND)`);
+         let (var,acc') = acc1 in
+          (Seq c1 (If (HD v1) (Seq c2 (Move var (HD v2)))
+                              (Seq c3 (Move var (HD v3)))),
+           [var],(var+1,acc'))) /\
+  (compile acc env tail [Let xs x2] =
+     let (c1,vs,acc1) = compile acc env F xs in
+     let (c2,v2,acc2) = compile acc1 (vs ++ env) tail [x2] in
+       (Seq c1 c2, v2, acc2)) /\
+  (compile acc env tail [Raise x1] =
+     let (c1,v1,acc1) = compile acc env F [x1] in
+       (Seq c1 (Raise (HD v1)), v1, acc1)) /\
+  (compile acc env tail [Op op xs] =
+     let (c1,vs,acc1) = compile acc env F xs in
+     let (c2,var,acc2) = compile_assign acc1 op (REVERSE vs) in
+     let c3 = Seq c1 c2 in
+       (if tail then Seq c3 (Return var) else c3, [var], acc2)) /\
+  (compile acc env tail [Tick x1] =
+     let (c1,v1,acc1) = compile acc env tail [x1] in
+       (Seq Tick c1, v1, acc1)) /\
+  (compile acc env tail [Call ticks dest xs NONE] =
+     let (c1,vs,acc1) = compile acc env F xs in
+     let (var,live:num_set,acc1') = acc1 in
+     let acc2 = (var+1:num,live,acc1') in
+     let ret = (if tail then NONE else SOME (var, live)) in
+       (Seq c1 (mk_ticks ticks (Call ret dest vs NONE)), [var], acc2)) /\
+  (compile acc env tail [Call ticks dest xs (SOME handler)] =
+     let (c1,vs,acc1) = compile acc env F xs in
+     let (var,live,acc1') = acc1 in
+     let acc2 = (var+2,live,acc1') in
+     let (c2,v,acc3) = compile acc2 (var::env) F [handler] in
+     let ret = SOME (var+1, live) in
+     let c3 = (if tail then Return (var+1) else Skip) in
+       (Seq c1 (mk_ticks ticks (Seq (Call ret dest vs
+                 (SOME (var,Seq c2 (Move (var+1) (HD v))))) c3)), [var+1], acc3))
+Termination
+  WF_REL_TAC ‘measure (exp2_size o SND o SND o SND)’
+End
 
-val compile_ind = theorem"compile_ind";
-
-val compile_LESS_EQ_lemma = Q.prove(
-  `!arch_size n env tail live xs.
-      n <= SND (SND (compile arch_size n env tail live xs))`,
-  HO_MATCH_MP_TAC compile_ind \\ REPEAT STRIP_TAC
-  \\ SIMP_TAC std_ss [compile_def] \\ SRW_TAC [] []
-  \\ FULL_SIMP_TAC (srw_ss()) [] \\ SRW_TAC [] [] \\ DECIDE_TAC);
-
-Theorem compile_LESS_EQ:
-   !arch_size n env tail live xs c vs new_var.
-      (compile arch_size n env tail live xs = (c,vs,new_var)) ==> n <= new_var
-Proof
-  REPEAT STRIP_TAC \\ MP_TAC (SPEC_ALL compile_LESS_EQ_lemma)
-  \\ FULL_SIMP_TAC std_ss []
-QED
-
-val compile_LENGTH_lemma = Q.prove(
-  `!arch_size n env tail live xs.
-      (LENGTH (FST (SND (compile arch_size n env tail live xs))) = LENGTH xs)`,
-  HO_MATCH_MP_TAC compile_ind \\ REPEAT STRIP_TAC
-  \\ SIMP_TAC std_ss [compile_def] \\ SRW_TAC [] []
-  \\ FULL_SIMP_TAC (srw_ss()) [] \\ SRW_TAC [] []);
+Definition compile_main_def:
+  compile_main arch_size arg_count e =
+    let env = COUNT_LIST arg_count in
+    let acc = (arg_count,fromAList (MAP (\n.(n,())) env),[],arch_size) in
+      FST (bvi_to_data$compile acc env T [e])
+End
 
 Theorem compile_LENGTH:
-   !arch_size n env tail live xs c vs new_var.
-      (compile arch_size n env tail live xs = (c,vs,new_var)) ==> (LENGTH vs = LENGTH xs)
+  !acc env tail xs c vs acc1.
+     (compile acc env tail xs = (c,vs,acc1)) ==> (LENGTH vs = LENGTH xs)
 Proof
-  REPEAT STRIP_TAC \\ MP_TAC (SPEC_ALL compile_LENGTH_lemma)
-  \\ FULL_SIMP_TAC std_ss []
+  recInduct compile_ind \\ rw []
+  \\ pop_assum mp_tac
+  \\ simp [Once compile_def]
+  \\ rpt (pairarg_tac \\ fs []) \\ rw[] \\ fs []
 QED
 
-Theorem compile_SING_IMP:
-   (compile arch_size n env tail live [x] = (c,vs,new_var)) ==> ?t. vs = [t]
+Theorem compile_SING:
+  (compile acc env tail [x] = (c,vs,acc1)) ==> ?t. vs = [t]
 Proof
-  REPEAT STRIP_TAC \\ IMP_RES_TAC compile_LENGTH
-  \\ Cases_on `vs` \\ FULL_SIMP_TAC (srw_ss()) []
-  \\ Cases_on `t` \\ FULL_SIMP_TAC (srw_ss()) []
+  rw [] \\ imp_res_tac compile_LENGTH
+  \\ fs [LENGTH_EQ_NUM_compute]
 QED
 
 (* combine dataLang optimisations *)
 
 val optimise_def = Define `
-  optimise arch_size prog = data_space$compile (simp (FST (data_live$compile prog LN arch_size)) Skip) arch_size`
+  optimise arch_size prog =
+    data_space$compile
+      (simp (FST (data_live$compile prog LN arch_size)) Skip) arch_size`
 
 (* the top-level compiler includes the optimisations, because the correctness
    proofs are combined *)
 
 val compile_exp = Define `
   compile_exp arch_size arg_count exp =
-    optimise arch_size (FST (compile arch_size arg_count (COUNT_LIST arg_count) T [] [exp]))`
+    optimise arch_size (compile_main arch_size arg_count exp)`
 
 val compile_part = Define `
   compile_part arch_size (name:num, arg_count, exp) =
@@ -188,5 +209,28 @@ val compile_part = Define `
 
 val compile_prog_def = Define `
   compile_prog arch_size prog = MAP (compile_part arch_size) prog`;
+
+(* tests
+
+val input1 =
+  “Let [Op El [Var 0; Op (Const 0) []] ;
+        Op El [Var 0; Op (Const 0) []]]
+     (Op (Cons 7) [Op (Const 0) []; Op (Const 0) []; Var 0; Var 1])”
+
+val input2 =
+  “If (Op (TagLenEq 0 0) [Op El [Var 0; Op (Const 0) []]])
+     (Var 1)
+     (If (Op (TagLenEq 0 0) [Op El [Op El [Var 0; Op (Const 0) []]; Op (Const 0) []]])
+       (Var 1) (Var 0))”
+
+fun test input =
+  EVAL “simp (compile_main 32 2 ^input) Skip”
+  |> SIMP_RULE (srw_ss()) [data_simpTheory.simp_def,data_simpTheory.pSeq_def]
+  |> CONV_RULE (RAND_CONV EVAL)
+
+val r1 = test input1;
+val r2 = test input2;
+
+*)
 
 val _ = export_theory();
